formal/FSet_Utils.thy
@@ -56,4 +56,7 @@ lemma filter_elements: "x |\<in>| Abs_fset (Set.filter f (fset s)) = (x \<in> (S
 
 lemma singleton_equiv: "is_singleton s \<Longrightarrow> (the_elem s = i) = (s = {i})"
   by (meson is_singleton_the_elem the_elem_eq)
+
+lemma sorted_list_of_empty [simp]: "sorted_list_of_fset {||} = []"
+  by (simp add: sorted_list_of_fset_def)
 end
