formal/Transition.thy
@@ -35,4 +35,10 @@ next
     by (simp add: \<open>Label x = Label y \<and> Arity x = Arity y \<and> Guard x = Guard y \<and> Outputs x = Outputs y \<and> Updates x = Updates y\<close>)
 qed
 
+lemma unequal_labels[simp]: "Label t1 \<noteq> Label t2 \<Longrightarrow> t1 \<noteq> t2"
+  by auto
+
+lemma unequal_arities[simp]: "Arity t1 \<noteq> Arity t2 \<Longrightarrow> t1 \<noteq> t2"
+  by auto
+
 end
